WIP: update case study with abstract state

io/case-study/Monitor.fst
@@ -2,12 +2,16 @@ module Monitor
 
 open FStar.ST
 open MIO.Sig
+open Utils
 
 private
-val h : ref trace
-let h = ST.alloc []
+val monitor_state : ref mymst.cst
+let monitor_state = ST.alloc mymst.init_cst
 
-let get_trace () : St trace = !h
+let get_state () : St mymst.cst = !monitor_state
 
-let update_trace (caller:bool) (cmd:io_cmds) (argz:io_sig.args cmd) (rez:io_sig.res cmd argz) : St unit =
-  h := (convert_call_to_event caller cmd argz rez) :: !h
+let update_state caller (cmd:io_cmds) (argz:io_sig.args cmd) (rez:io_sig.res cmd argz) : St unit =
+  let s0 = get_state () in
+  let e = convert_call_to_event caller cmd argz rez in
+  let s1 = mymst.update_cst s0 e in
+  monitor_state := s1
