io/case-study/AdversarialHandlers.fst
@@ -46,4 +46,4 @@ let main3 : comp.target.whole = comp.target.link compiled_webserver handler3
 let main4 : comp.target.whole = comp.target.link compiled_webserver handler4
 let main5 : comp.target.whole = comp.target.link compiled_webserver handler5
 
-let _ = Execute.execute main5._22
+let _ = Execute.execute main5._2
